PiLL/PiLL/Framework/Model/Base.lean
@@ -36,8 +36,8 @@ notation:max S:max "⸨" R "⸩" => HasOpen.open_ S R 0
 class HasClose (Subject Replacement Target : Type) where
   close_ : Subject → Replacement → Target → Subject
 
-notation:max S:max "⟦" T " | " R "⟧" => HasOpen.close_ S R T
-notation:max S:max "⟦" R "⟧" => HasOpen.close_ S R 0
+notation:max S:max "⟪" T " | " R "⟫" => HasClose.close_ S R T
+notation:max S:max "⟪" R "⟫" => HasClose.close_ S R 0
 
 class HasOpenTwo (Subject Replacement_1 Replacement_2 Target : Type) where
   open_ : Subject → Replacement_1 → Replacement_2 → Target → Subject
@@ -48,8 +48,8 @@ notation:max S:max "⸨" R1 ", " R2 "⸩" => HasOpenTwo.open_ S R1 R2 0
 class HasCloseTwo (Subject Replacement_1 Replacement_2 Target : Type) where
   close_ : Subject → Replacement_1 → Replacement_2 → Target → Subject
 
-notation:max S:max "⟦" T " | " R1 ", " R2 "⟧" => HasOpenTwo.open_ S R1 R2 T
-notation:max S:max "⟦" R1 ", " R2 "⟧" => HasOpenTwo.open_ S R1 R2 0
+notation:max S:max "⟪" T " | " R1 ", " R2 "⟫" => HasCloseTwo.close_ S R1 R2 T
+notation:max S:max "⟪" R1 ", " R2 "⟫" => HasCloseTwo.close_ S R1 R2 0
 
 class HasBracket (Subject Content Result : Type) where
    brack : Subject → Content → Result
